parser/Utils.v
@@ -351,10 +351,9 @@ Lemma fold_left_preserves_list_invar' :
     eexists; apply in_or_app; left; eauto.
   Qed.
 
-
   Lemma heads_eq_tails_eq__lists_eq :
     forall (A : Type) (x y : A) (xs ys : list A),
       x = y -> xs = ys -> x :: xs = y :: ys.
   Proof.
     intros; subst; auto.
-  Qed. 
+  Qed.
